KeyManagement/Simulation.v
@@ -1,8 +1,11 @@
 From Coq Require Import
      List
-     Eqdep.
+     Eqdep
+     Program.Equality (* for dependent induction *)
+.
 
-Require Import MyPrelude Users Common. 
+
+Require Import MyPrelude Users Common MapLtac. 
 
 Require IdealWorld
         RealWorld.
@@ -21,8 +24,8 @@ Ltac invert H :=
 
 Hint Resolve in_eq in_cons.
 
-Definition rstepSilent {A : Type} (U1 U2 : RealWorld.universe A) :=
-  RealWorld.lstep_universe U1 Silent U2.
+Definition rstepSilent {A B : Type} (U1 U2 : RealWorld.universe A B) :=
+  RealWorld.step_universe U1 Silent U2.
 
 Definition istepSilent {A : Type} (U1 U2 : IdealWorld.universe A) :=
   IdealWorld.lstep_universe U1 Silent U2.
@@ -97,9 +100,9 @@ Inductive action_matches :
     -> action_matches rw iw
 .
 
-Definition lsimulates {A : Type}
-           (R : RealWorld.universe A -> IdealWorld.universe A -> Prop)
-           (U__r : RealWorld.universe A) (U__i : IdealWorld.universe A) :=
+Definition simulates {A B : Type}
+           (R : RealWorld.universe A B -> IdealWorld.universe A -> Prop)
+           (U__r : RealWorld.universe A B) (U__i : IdealWorld.universe A) :=
 
 (*  call spoofable *)
 
@@ -114,7 +117,7 @@ Definition lsimulates {A : Type}
   /\ (forall U__r U__i,
         R U__r U__i
         -> forall a1 U__r',
-          RealWorld.lstep_universe U__r (Action a1) U__r' (* excludes adversary steps *)
+          RealWorld.step_universe U__r (Action a1) U__r' (* excludes adversary steps *)
           -> exists a2 U__i' U__i'',
             istepSilent^* U__i U__i'
             /\ IdealWorld.lstep_universe U__i' (Action a2) U__i''
@@ -126,20 +129,308 @@ Definition lsimulates {A : Type}
 
   /\ R U__r U__i.
 
-Definition lrefines {A : Type} (U1 : RealWorld.universe A)(U2 : IdealWorld.universe A) :=
-  exists R, lsimulates R U1 U2.
+Definition refines {A B : Type} (U1 : RealWorld.universe A B)(U2 : IdealWorld.universe A) :=
+  exists R, simulates R U1 U2.
 
-Infix "<|" := lrefines (no associativity, at level 70).
+Infix "<|" := refines (no associativity, at level 70).
 
 
-Inductive couldGenerate : forall {A}, RealWorld.universe A -> list RealWorld.action -> Prop :=
-| CgNothing : forall {A} (u : RealWorld.universe A),
-    couldGenerate u []
-| CgSilent : forall {A} {u u' : RealWorld.universe A} tr,
-    RealWorld.lstep_universe u Silent u'
-    -> couldGenerate u' tr
-    -> couldGenerate u tr
-| CgAction : forall {A} a (u u' : RealWorld.universe A) tr,
-    RealWorld.lstep_universe u (Action a) u'
-    -> couldGenerate u' tr
-    -> couldGenerate u (a :: tr).
+(* Inductive couldGenerate : forall {A B}, RealWorld.universe A B -> list RealWorld.action -> Prop := *)
+(* | CgNothing : forall {A B} (u : RealWorld.universe A), *)
+(*     couldGenerate u [] *)
+(* | CgSilent : forall {A} {u u' : RealWorld.universe A} tr, *)
+(*     RealWorld.lstep_universe u Silent u' *)
+(*     -> couldGenerate u' tr *)
+(*     -> couldGenerate u tr *)
+(* | CgAction : forall {A} a (u u' : RealWorld.universe A) tr, *)
+(*     RealWorld.lstep_universe u (Action a) u' *)
+(*     -> couldGenerate u' tr *)
+(*     -> couldGenerate u (a :: tr). *)
+
+
+Section SingleAdversarySimulates.
+
+  (* If we have a simulation proof, we know that:
+   *   1) No receives could have accepted spoofable messages
+   *   2) Sends we either of un-spoofable, or were 'public' and are safely ignored
+   *
+   * This should mean we can write some lemmas that say we can:
+   *   safely ignore all adversary messages (wipe them from the universe) -- Adam's suggestion, I am not exactly sure how...
+   *   or, prove an appended simulation relation, but I am not sure how to generically express this
+   *)
+
+  Definition ADV := 10.
+
+  Definition add_adversary {A B} (U__r : RealWorld.universe A B) (advcode : RealWorld.user_cmd B) :=
+    RealWorld.addAdversaries U__r ($0 $+ (ADV, {| RealWorld.key_heap := $0
+                                              ; RealWorld.msg_heap := []
+                                              ; RealWorld.protocol := advcode |})).
+
+  Definition strip_adversary {A B} (U__r : RealWorld.universe A B) : RealWorld.universe A B :=
+    {| RealWorld.users       := U__r.(RealWorld.users)
+     ; RealWorld.adversary   := $0
+     ; RealWorld.all_ciphers := U__r.(RealWorld.all_ciphers)
+     |}.
+
+
+  (* Lemma adversary_univ_loud_step_implies_stripped_nonadv_step : *)
+  (*   forall {A B} (U__r U__ra : RealWorld.universe A B) advcode, *)
+  (*       U__ra = add_adversary U__r advcode *)
+  (*     -> U__r.(RealWorld.adversary) = $0 *)
+  (*     -> forall U__r' U__ra' a, *)
+  (*         RealWorld.lstep_universe U__ra (Action a) U__ra' *)
+  (*       -> U__r' = strip_adversary U__ra' *)
+  (*       -> RealWorld.lstep_universe U__r (Action a) U__r'. *)
+  (* Proof. *)
+  (*   intros. *)
+  (*   invert H1. *)
+  (*   invert H4. *)
+
+  (*   (* Bind *) *)
+  (*   - admit. *)
+
+  (*   (* Recv *) *)
+  (*   - eapply RealWorld.LStepUser'; eauto. *)
+  (*     unfold RealWorld.universe_data_step; simpl. *)
+  (*     match goal with *)
+  (*     | [ H : _ = RealWorld.protocol _ |- _ ] => rewrite <- H *)
+  (*     end. *)
+  (*     eapply RealWorld.LStepRecv'; eauto. *)
+  (*     unfold strip_adversary, RealWorld.updateUniverse; simpl. *)
+  (*     eapply real_univ_eq_fields_eq; auto. *)
+
+  (*   (* Send *) *)
+  (*   - eapply RealWorld.LStepUser'; eauto. *)
+  (*     unfold RealWorld.universe_data_step; simpl. *)
+  (*     match goal with *)
+  (*     | [ H : _ = RealWorld.protocol _ |- _ ] => rewrite <- H *)
+  (*     end. *)
+  (*     eapply RealWorld.LStepSend; eauto. *)
+  (*     unfold RealWorld.updateUniverse, strip_adversary; simpl. *)
+  (*     rewrite H0.  *)
+  (*     smash_universe. *)
+  (* Admitted. *)
+
+
+  Lemma honest_step_advuniv_implies_honest_step_origuniv :
+    forall {A B} (U__r : RealWorld.universe A B) u_id userData advcode gs adv adv' uks cmd,
+      RealWorld.step_user u_id Silent (RealWorld.build_data_step (add_adversary U__r advcode) userData) (gs, adv, uks, cmd)
+      -> U__r.(RealWorld.adversary) = $0
+      -> RealWorld.users (add_adversary U__r advcode) $? u_id = Some userData
+      -> adv' = $0
+      -> RealWorld.step_user u_id Silent (RealWorld.build_data_step U__r userData) (gs, adv', uks, cmd).
+  Proof.
+    intros.
+    invert H.
+    - admit.
+    - admit.
+    - unfold RealWorld.build_data_step. 
+
+  Admitted.
+
+  Section RealWorldLemmas.
+    Import RealWorld.
+
+    Lemma univ_components :
+      forall {A B} (U__r : universe A B),
+        {| users       := users U__r
+         ; adversary   := adversary U__r
+         ; all_ciphers := all_ciphers U__r
+        |} = U__r.
+      intros. destruct U__r; simpl; trivial.
+    Qed.
+
+    Lemma adduserkeys_keys_idempotent :
+      forall {A} (us : user_list (user_data A)) ks uid ud,
+        us $? uid = Some ud
+        -> exists ud', addUserKeys us ks $? uid = Some ud'.
+    Proof.
+      intros.
+      (* eexists. *)
+      unfold addUserKeys.
+      apply find_mapsto_iff in H.
+      eexists.
+      rewrite <- find_mapsto_iff.
+      rewrite map_mapsto_iff.
+      eexists; intuition. eassumption.
+    Qed.
+  End RealWorldLemmas.
+
+  Hint Constructors RealWorld.step_user.
+
+  Hint Extern 1 (rstepSilent _ (strip_adversary _)) => 
+    unfold RealWorld.buildUniverse, RealWorld.buildUniverseAdv, strip_adversary,
+           updateUserList, RealWorld.findUserKeys;
+      simpl.
+
+  Hint Extern 1 (rstepSilent _ _) => eapply RealWorld.StepUser.
+  Hint Extern 1 (RealWorld.step_user _ _ (RealWorld.build_data_step _ _) _) =>
+    progress unfold RealWorld.build_data_step.
+
+  Hint Extern 1 (RealWorld.step_user _ _ (_, _, _ , RealWorld.protocol _) _) => 
+    match goal with
+    | [ H : _ = RealWorld.protocol _ |- _ ] => rewrite <- H
+    end.
+
+  Hint Extern 1 (_ = _) => progress m_equal.
+  Hint Extern 1 (_ = _) => progress f_equal.
+  Hint Extern 1 (_ = _) =>
+    progress unfold RealWorld.build_data_step, RealWorld.buildUniverse, updateUserList; simpl.
+  Hint Extern 1 (_ = _) =>
+    match goal with
+    | [ H : RealWorld.adversary _ = _ |- _ ] => rewrite <- H
+    end.
+  Hint Extern 1 (_ = RealWorld.adversary _) => solve [ symmetry ; assumption ].
+
+
+  (* Lemma simulates_with_adversary_silent : *)
+  (*  forall {A B} (U__r : RealWorld.universe A B) (U__i : IdealWorld.universe A) R, *)
+  (*      simulates R U__r U__i *)
+  (*    -> U__r.(RealWorld.adversary) = $0 *)
+  (*    -> forall U__ra U__ra' advcode, *)
+  (*        U__ra = add_adversary U__r advcode *)
+  (*        -> rstepSilent U__ra U__ra' *)
+  (*        -> exists U__i', *)
+  (*            istepSilent ^* U__i U__i' *)
+  (*            /\ R (strip_adversary U__ra') U__i'. *)
+  (*  Proof. *)
+  (*    intros. *)
+  (*    inversion H  as [H__silent H__l]; clear H. *)
+  (*    inversion H__l as [H__loud R__start]; clear H__l; clear H__loud. *)
+
+  (*    invert H2. *)
+  
+  (*    (* Honest step *)  *)
+  (*    - invert H3; unfold RealWorld.build_data_step; simpl; *)
+  (*        [ | specialize (H__silent U__r U__i R__start); eapply H__silent .. ]; *)
+  (*        eauto 9. *)
+  (*      + admit. *)
+  
+  (*    (* Adversary step *)  *)
+  (*    - invert H3; unfold RealWorld.build_data_step; simpl; *)
+  (*        [ | unfold strip_adversary, RealWorld.buildUniverseAdv, updateUserList; *)
+  (*              simpl; *)
+  (*              exists U__i; *)
+  (*              rewrite <- H0; *)
+  (*              try rewrite univ_components; *)
+  (*              intuition .. *)
+  (*        ]. *)
+
+  (*      + admit. *)
+  (*      + admit. (* need to swipe ciphers *) *)
+  (*      + admit. (* need to swipe ciphers *) *)
+  
+  (*  Admitted. *)
+  
+  Lemma simulates_with_adversary_silent :
+    forall {A B} (U__ra : RealWorld.universe A B) (U__i : IdealWorld.universe A) R,
+      simulates R (strip_adversary U__ra) U__i
+      -> forall U__ra',
+        rstepSilent U__ra U__ra'
+        -> exists U__i',
+          istepSilent ^* U__i U__i'
+          /\ R (strip_adversary U__ra') U__i'.
+  Proof.
+    intros.
+    inversion H  as [H__silent H__l]; clear H.
+    inversion H__l as [H__loud R__start]; clear H__l; clear H__loud.
+
+    invert H0.
+
+    (* Honest step *) 
+    - invert H1; unfold RealWorld.build_data_step; simpl;
+        [ | specialize (H__silent (strip_adversary U__ra) U__i R__start); eapply H__silent .. ];
+        eauto 9.
+      + admit.
+
+    (* Adversary step *) 
+    - invert H1; unfold RealWorld.build_data_step; simpl; [
+        | unfold strip_adversary, RealWorld.buildUniverseAdv, updateUserList;
+            simpl;
+            exists U__i;
+            match goal with | [ H : R (strip_adversary _) _ |- _ ] => progress unfold strip_adversary in H; simpl in H end;
+            intuition ..
+        ].
+
+        + admit.
+        + admit. (* something with send.. *)
+        + admit. (* need to swipe ciphers *)
+        + admit. (* need to swipe ciphers *)
+
+    Admitted.
+
+    Lemma simulates_with_adversary_loud :
+      forall {A B} (U__ra : RealWorld.universe A B) (U__i : IdealWorld.universe A) R,
+        simulates R (strip_adversary U__ra) U__i
+        -> forall U__ra' a__ra,
+          RealWorld.step_universe U__ra (Action a__ra) U__ra' (* excludes adversary steps *)
+          -> exists a__i U__i' U__i'',
+              istepSilent^* U__i U__i'
+            /\ IdealWorld.lstep_universe U__i' (Action a__i) U__i''
+            /\ action_matches a__ra a__i
+            /\ R (strip_adversary U__ra') U__i''
+            /\ RealWorld.action_adversary_safe (RealWorld.findUserKeys U__ra.(RealWorld.adversary)) a__ra = true.
+    Proof.
+
+      intros.
+      inversion H  as [H__silent H__l]; clear H.
+      inversion H__l as [H__loud R__start]; clear H__l; clear H__silent.
+
+      match goal with
+      | [ H : RealWorld.step_universe _ _ _ |- _] => invert H
+      end.
+
+      match goal with
+      | [ H : RealWorld.step_user _ _ _ _ |- _] => invert H
+      end; 
+        unfold RealWorld.build_data_step; simpl;
+          [ | specialize (H__loud (strip_adversary U__ra) U__i R__start) ..
+          ].
+
+      - admit.
+      - admit.
+      - admit.
+
+      (* - unfold RealWorld.buildUniverse, updateUserList; simpl. *)
+      (*   unfold RealWorld.findUserKeys,fold in H__loud; simpl in H__loud. *)
+      (*   eapply H__loud. *)
+
+      (* (* Hint Extern 1 (step_universe _ _ _) => eapply RealWorld.StepUser. *) *)
+
+      (* - simpl in *. *)
+      (*   unfold strip_adversary, RealWorld.buildUniverse, updateUserList; simpl. *)
+      (*   eapply RealWorld.StepUser; eauto. *)
+
+      (* - simpl in *. *)
+      (*   unfold strip_adversary, RealWorld.buildUniverse, updateUserList; simpl. *)
+      (*   eapply RealWorld.StepUser. exact H. eauto. *)
+      (*   unfold RealWorld.buildUniverse, updateUserList; simpl. *)
+      (*   rewrite H0; smash_universe. *)
+
+    Admitted.
+
+
+  Theorem simulates_ok_with_adversary :
+    forall {A B} (U__r : RealWorld.universe A B) (U__i : IdealWorld.universe A),
+      U__r <| U__i
+      -> U__r.(RealWorld.adversary) = $0
+      -> forall U__ra advcode,
+          U__ra = add_adversary U__r advcode
+          -> U__ra <| U__i.
+  Proof.
+    intros.
+    inversion H as [R SIM].
+    inversion SIM as [H__silent H__l].
+    inversion H__l as [H__loud R__start]; clear H__l.
+
+    unfold refines.
+    exists (fun ur ui => R (strip_adversary ur) ui); unfold simulates.
+    propositional.
+    - eapply simulates_with_adversary_silent; eauto. unfold simulates; eauto.
+    - eapply simulates_with_adversary_loud; eauto. unfold simulates; eauto.
+    - rewrite H1;
+        unfold strip_adversary, add_adversary; simpl;
+          rewrite <- H0; rewrite univ_components; eauto.
+  Qed.
+
+End SingleAdversarySimulates.
