KeyManagement/MapLtac.v
@@ -1,51 +1,40 @@
 From Coq Require Import
      List
-     Logic.ProofIrrelevance.
+     Logic.ProofIrrelevance
+     Program.Equality.
 
 Require Import MyPrelude.
-Require Import Users Common Simulation.
-Require RealWorld.
+Require Import Users Common.
+Require IdealWorld RealWorld.
 
 Import IdealWorld.IdealNotations
        RealWorld.RealWorldNotations.
 
 Section RealLemmas.
 
+  Import RealWorld.
+
   Lemma real_univ_eq_fields_eq :
-    forall {A} (us us' : user_list (RealWorld.user_data A)) a a' ud ud',
+    forall {A B} (us us' : honest_users A) (a a' : adversaries B) ud ud',
       us = us'
       -> a = a'
       -> ud = ud'
-      -> {| RealWorld.users := us
-         ; RealWorld.adversary := a
-         ; RealWorld.univ_data := ud
+      -> {| users := us
+         ; adversary := a
+         ; all_ciphers := ud
         |} =
-        {| RealWorld.users := us'
-         ; RealWorld.adversary := a'
-         ; RealWorld.univ_data := ud'
-        |}.
-  Proof.
-    intros; subst; reflexivity.
-  Qed.
-
-  Lemma real_ud_eq_fields_eq :
-    forall um um' ks ks' cs cs',
-        um = um'
-      -> ks = ks'
-      -> cs = cs'
-      -> {| RealWorld.users_msg_buffer := um;
-           RealWorld.all_keys         := ks;
-           RealWorld.all_ciphers      := cs
-        |} =
-        {| RealWorld.users_msg_buffer := um';
-           RealWorld.all_keys         := ks';
-           RealWorld.all_ciphers      := cs'
+        {| users := us'
+         ; adversary := a'
+         ; all_ciphers := ud'
         |}.
   Proof.
     intros; subst; reflexivity.
   Qed.
 
 End RealLemmas.
+
+Module Import OTF := OrderedType.OrderedTypeFacts OrderedTypeEx.Nat_as_OT.
+Module Import OMF := FSets.FMapFacts.OrdProperties NatMap.
 
 Section MapLemmas.
 
@@ -56,13 +45,159 @@ Section MapLemmas.
   Proof.
     intros; subst; f_equal; apply proof_irrelevance.
   Qed.
-  
+
+  Lemma map_eq_elements_eq :
+    forall {V} (m m' : NatMap.t V),
+      elements m = elements m'
+      -> m = m'.
+  Proof.
+    intros. destruct m. destruct m'.
+    simpl in *;
+      eapply map_eq_fields_eq;
+      eauto.
+  Qed.
+
+  Lemma Equal_hd_tl :
+    forall {V} (m1 m1' m2 m2' : t V) x xs y ys sx sy,
+        m1 = {| this := x :: xs ; sorted := sx |}
+      -> m2 = {| this := y :: ys ; sorted := sy |}
+      -> Equal m1 m2
+      -> m1' = m1 $- fst x
+      -> m2' = m2 $- fst y
+      -> x = y /\ Equal m1' m2'.
+  Proof.
+    intros.
+
+    destruct x as [n1 v1]; destruct y as [n2 v2]; simpl in *.
+
+    assert ( (n1,v1) = (n2,v2) ).
+    - unfold Equal in H1; subst; simpl in *.
+      unfold Equal in H1.
+      pose proof H1 as HH1; pose proof H1 as HH2.
+      specialize (HH1 n1); specialize (HH2 n2).
+      unfold find, Raw.find in HH1, HH2; simpl in *.
+      
+      pose proof (Raw.MX.elim_compare_eq) as EQn1.
+      pose proof (Raw.MX.elim_compare_eq) as EQn2.
+      specialize (EQn1 n1 n1 (eq_refl n1)); specialize (EQn2 n2 n2 (eq_refl n2)).
+      destruct EQn1, EQn2. rewrite H in *; rewrite H0 in *; clear x H x0 H0.
+
+      cases (OrderedTypeEx.Nat_as_OT.compare n1 n2).
+      + invert HH1.
+      + unfold OrderedTypeEx.Nat_as_OT.eq in e; invert HH1; trivial.
+      + cases (OrderedTypeEx.Nat_as_OT.compare n2 n1).
+        * invert HH2.
+        * unfold OrderedTypeEx.Nat_as_OT.eq in e; invert HH2; trivial. (* hokey proof -- shorter than deriving the contradiction *)
+        * unfold OrderedTypeEx.Nat_as_OT.lt in l; unfold OrderedTypeEx.Nat_as_OT.lt in l0.
+          assert (LT : n1 < n2) by assumption; apply lt_le in LT; contradiction.
+
+    - constructor; auto.
+
+      subst.
+
+      pose proof (Raw.MX.elim_compare_eq) as EQn2.
+      specialize (EQn2 n2 n2 (eq_refl n2)).
+      destruct EQn2.
+      unfold Equal in *; simpl in *.
+
+      intro k; invert H4.
+      case (k ==n n2); intros; subst.
+      + rewrite remove_eq_o by apply eq_refl.
+        rewrite remove_eq_o by apply eq_refl.
+        auto.
+      + rewrite remove_neq_o by auto.
+        rewrite remove_neq_o by auto.
+        specialize (H1 k); assumption.
+  Qed.
+
+
+  Lemma remove_hd :
+    forall {V} n (v : V) xs sx hdrel,
+      {| this := (n,v) :: xs ; sorted := Sorted.Sorted_cons sx hdrel |} $- n = {| this := xs ; sorted := sx |}.
+  Proof.
+    intros.
+    unfold remove, Raw.remove. simpl.
+    eapply map_eq_elements_eq; simpl.
+
+    pose proof (Raw.MX.elim_compare_eq) as EQn; specialize (EQn n n (eq_refl n)); destruct EQn.
+    rewrite H; trivial.
+  Qed.
+
+  Lemma map_eq_Equal :
+    forall {V} (m m' : t V),
+      Equal m m'
+      -> m = m'.
+  Proof.
+
+    intro V.
+    intro m.
+    destruct m as [l sl].
+    generalize dependent l.
+    induction l; intros.
+
+    - unfold Equal in H. simpl in *.
+      symmetry in H.
+      apply map_eq_elements_eq; simpl.
+
+      destruct m'; simpl in *.
+      cases this0.
+      + trivial.
+      + intros. destruct p. specialize (H n).
+        unfold find, Raw.find in H; simpl in H.
+        (* assert (n = n) by trivial. *)
+        
+        pose proof (Raw.MX.elim_compare_eq).
+        specialize (H0 n n (eq_refl n)).
+        destruct H0.
+        rewrite H0 in H.
+        invert H.
+
+    - simpl.
+      destruct m'; cases this0; simpl in *.
+      + destruct a as [n v].
+        unfold Equal in H; specialize (H n).
+        unfold find, Raw.find in H; simpl in H.
+        pose proof (Raw.MX.elim_compare_eq) as P; specialize (P n n (eq_refl n)); destruct P.
+        rewrite H0 in H; invert H.
+
+      + destruct a as [n1 v1]; destruct p as [n2 v2].
+        eapply Equal_hd_tl in H; eauto.
+        destruct H; invert H.
+        unfold Equal in H0; simpl in *.
+
+        dependent destruction sl.
+        dependent destruction sorted0.
+        specialize (IHl sl {| this := this0 ; sorted := sorted0 |}).
+
+        assert (tlEQ : Equal {| this := l ; sorted := sl |} {| this := this0 ; sorted := sorted0 |} ).
+        * unfold Equal; intro k; specialize (H0 k); do 2 rewrite remove_hd in H0; assumption.
+        * specialize (IHl tlEQ).
+          dependent destruction IHl.
+          eapply map_eq_elements_eq; simpl; f_equal.
+  Qed.
+
   Lemma add_empty_idempotent :
     forall V (m : NatMap.t V),
       m $++ $0 = m.
   Proof.
     intros; unfold merge_maps, fold, Raw.fold; simpl; auto.
   Qed.
+
+  Lemma empty_add_idempotent : 
+    forall V (m : NatMap.t V),
+      $0 $++ m = m.
+  Proof.
+    intros; unfold merge_maps.
+    apply P.fold_rec.
+    - intros.
+      apply elements_Empty in H.
+      apply map_eq_elements_eq. auto.
+      
+    - intros. subst.
+      apply map_eq_Equal. unfold Equal; intros.
+      unfold P.Add in H1. specialize (H1 y). symmetry; auto.
+  Qed.
+
 
 End MapLemmas.
 
@@ -71,28 +206,25 @@ Ltac m_equal :=
          (* | [ |- context[find ?k (add ?k' _ _) ] ] => idtac k; idtac k'; case (eq_dec k k'); intro *)
          | [ |- context[find ?k (add ?k _ _) ] ] => rewrite add_eq_o by (simple apply @eq_refl)
          | [ |- context[find ?k (add ?k' _ _) ] ] => rewrite add_neq_o by discriminate
+         | [ |- context[$0 $++ _ ] ] => rewrite empty_add_idempotent
+         | [ |- context[_ $++ $0 ] ] => rewrite add_empty_idempotent
          | [ |- (add _ _ _) = _ ] => normalize_set
          | [ |- (add _ _ _) = _ ] => unfold add, Raw.add; simpl
          | [ |- empty _ = _ ] => unfold empty, Raw.empty, remove, Raw.remove; simpl
          | [ |- {| this := _ ; sorted := _ |} = _ ] => eapply map_eq_fields_eq
          end.
 
-Hint Rewrite add_empty_idempotent : maps.
-  
+Hint Rewrite add_empty_idempotent empty_add_idempotent : maps.
+
 Ltac smash_universe :=
-  unfold RealWorld.updateUniverse, updateUserList;
+  unfold RealWorld.buildUniverse, updateUserList;
   repeat (match goal with
           | [ |- {| RealWorld.users := _
-                   ; RealWorld.adversary := _
-                   ; RealWorld.univ_data := _ |} = _
+                 ; RealWorld.adversary := _
+                 ; RealWorld.all_ciphers := _ |} = _
             ] => eapply real_univ_eq_fields_eq
-          | [ |- {| RealWorld.users_msg_buffer := _
-                   ; RealWorld.all_keys         := _
-                   ; RealWorld.all_ciphers      := _ |} = _
-            ] => eapply real_ud_eq_fields_eq
           | [ |- _ = _ ] => reflexivity
           end; m_equal).
-
 
 Section ExamplarProofs.
 
@@ -116,79 +248,79 @@ Section ExamplarProofs.
     Definition B__keys := $0 $+ (KID1, AsymKey KEY1 false) $+ (KID2, AsymKey KEY2 true).
   End RealProtocolParams.
 
-  Lemma ex1: forall cid1 (n : nat) cs, exists qn qcid1 qcs,
-    (RealWorld.updateUniverse
-       {| RealWorld.users := $0 $+ (A,
-          {| RealWorld.key_heap := A__keys;
-             RealWorld.protocol :=
-               (_  <- RealWorld.Return tt;
-                m' <- @RealWorld.Recv (RealWorld.Pair RealWorld.Nat RealWorld.CipherId) (RealWorld.Signed KID2 RealWorld.Accept);
-                RealWorld.Return
-                  match RealWorld.unPair m' with
-                  | Some (RealWorld.Plaintext n', _) =>
-                    if qn ==n n' then true else false
-                  | _ => false
-                  end)%realworld |}) $+ (B,
-          {| RealWorld.key_heap := B__keys;
-             RealWorld.protocol :=
-               (m  <- RealWorld.Return (RealWorld.Signature (RealWorld.Plaintext qn) qcid1);
-                v  <- RealWorld.Verify (RealWorld.AsymKey KEY1 false) m;
-                m' <- match RealWorld.unPair m with
-                     | Some (p, _) => RealWorld.Sign KEY__B p
-                     | None => RealWorld.Sign KEY__B (RealWorld.Plaintext 1)
-                     end; _ <- RealWorld.Send A m'; RealWorld.Return v)%realworld |});
-          RealWorld.adversary := $0;
-          RealWorld.univ_data :=
-            {|
-              RealWorld.users_msg_buffer := $0;
-              RealWorld.all_keys := KEYS;
-              RealWorld.all_ciphers :=
-                qcs $+ (qcid1,
-                        RealWorld.Cipher qcid1 KID1 (RealWorld.Plaintext qn)) |} |}
-       {| RealWorld.users_msg_buffer := $0;
-          RealWorld.all_keys := KEYS;
-          RealWorld.all_ciphers := qcs $+ (qcid1, RealWorld.Cipher qcid1 KID1 (RealWorld.Plaintext qn)) |} $0 A A__keys
-       (m' <- @RealWorld.Recv (RealWorld.Pair RealWorld.Nat RealWorld.CipherId) (RealWorld.Signed KID2 RealWorld.Accept);
-        RealWorld.Return
-          match RealWorld.unPair m' with
-          | Some (RealWorld.Plaintext n', _) => if qn ==n n' then true else false
-          | _ => false
-          end)%realworld) = 
-       {| RealWorld.users := $0 $+ (A,
-          {| RealWorld.key_heap := A__keys;
-             RealWorld.protocol :=
-               (m' <- @RealWorld.Recv (RealWorld.Pair RealWorld.Nat RealWorld.CipherId) (RealWorld.Signed KID2 RealWorld.Accept);
-                RealWorld.Return
-                  match RealWorld.unPair m' with
-                  | Some (RealWorld.Plaintext n', _) => if n ==n n' then true else false
-                  | _ => false
-                  end)%realworld |}) $+ (B,
-          {| RealWorld.key_heap := B__keys;
-             RealWorld.protocol :=
-               (m <- RealWorld.Recv (RealWorld.Signed KID1 RealWorld.Accept);
-                v <- RealWorld.Verify (RealWorld.AsymKey KEY1 false) m;
-                m' <- match RealWorld.unPair m with
-                     | Some (p, _) => RealWorld.Sign KEY__B p
-                     | None => RealWorld.Sign KEY__B (RealWorld.Plaintext 1)
-                     end; _ <- RealWorld.Send A m'; RealWorld.Return v)%realworld |}) $+ (B,
-          {| RealWorld.key_heap := B__keys $++ $0;
-             RealWorld.protocol :=
-               (m <- RealWorld.Return (RealWorld.Signature (RealWorld.Plaintext n) cid1);
-                v <- RealWorld.Verify (RealWorld.AsymKey KEY1 false) m;
-                m' <- match RealWorld.unPair m with
-                     | Some (p, _) => RealWorld.Sign KEY__B p
-                     | None => RealWorld.Sign KEY__B (RealWorld.Plaintext 1)
-                     end; _ <- RealWorld.Send A m'; RealWorld.Return v)%realworld |});
-          RealWorld.adversary := $0;
-          RealWorld.univ_data :=
-            {| RealWorld.users_msg_buffer :=
-                 $0 $+ (B, [Exm (RealWorld.Signature (RealWorld.Plaintext n) cid1)]) $- B;
-               RealWorld.all_keys := KEYS;
-               RealWorld.all_ciphers := cs $+ (cid1, RealWorld.Cipher cid1 KID1 (RealWorld.Plaintext n)) |}
-       |}
-  .
-  Proof.
-    intros; do 3 eexists. smash_universe.
-  Qed.
+  (* Lemma ex1: forall {AT : Type} cid1 (n : nat) cs, exists qn qcid1 qcs, *)
+  (*   (RealWorld.updateUniverse *)
+  (*      {| RealWorld.users := $0 $+ (A, *)
+  (*         {| RealWorld.key_heap := A__keys; *)
+  (*            RealWorld.protocol := *)
+  (*              (_  <- RealWorld.Return tt; *)
+  (*               m' <- @RealWorld.Recv (RealWorld.Pair RealWorld.Nat RealWorld.CipherId) (RealWorld.Signed KID2 RealWorld.Accept); *)
+  (*               RealWorld.Return *)
+  (*                 match RealWorld.unPair m' with *)
+  (*                 | Some (RealWorld.Plaintext n', _) => *)
+  (*                   if qn ==n n' then true else false *)
+  (*                 | _ => false *)
+  (*                 end)%realworld |}) $+ (B, *)
+  (*         {| RealWorld.key_heap := B__keys; *)
+  (*            RealWorld.protocol := *)
+  (*              (m  <- RealWorld.Return (RealWorld.Signature (RealWorld.Plaintext qn) qcid1); *)
+  (*               v  <- RealWorld.Verify (RealWorld.AsymKey KEY1 false) m; *)
+  (*               m' <- match RealWorld.unPair m with *)
+  (*                    | Some (p, _) => RealWorld.Sign KEY__B p *)
+  (*                    | None => RealWorld.Sign KEY__B (RealWorld.Plaintext 1) *)
+  (*                    end; _ <- RealWorld.Send A m'; RealWorld.Return v)%realworld |}); *)
+  (*         RealWorld.adversary := ($0 : RealWorld.adversaries AT); *)
+  (*         RealWorld.univ_data := *)
+  (*           {| *)
+  (*             RealWorld.users_msg_buffer := $0; *)
+  (*             RealWorld.all_keys := KEYS; *)
+  (*             RealWorld.all_ciphers := *)
+  (*               qcs $+ (qcid1, *)
+  (*                       RealWorld.Cipher qcid1 KID1 (RealWorld.Plaintext qn)) |} |} *)
+  (*      {| RealWorld.users_msg_buffer := $0; *)
+  (*         RealWorld.all_keys := KEYS; *)
+  (*         RealWorld.all_ciphers := qcs $+ (qcid1, RealWorld.Cipher qcid1 KID1 (RealWorld.Plaintext qn)) |} $0 A A__keys *)
+  (*      (m' <- @RealWorld.Recv (RealWorld.Pair RealWorld.Nat RealWorld.CipherId) (RealWorld.Signed KID2 RealWorld.Accept); *)
+  (*       RealWorld.Return *)
+  (*         match RealWorld.unPair m' with *)
+  (*         | Some (RealWorld.Plaintext n', _) => if qn ==n n' then true else false *)
+  (*         | _ => false *)
+  (*         end)%realworld) =  *)
+  (*      {| RealWorld.users := $0 $+ (A, *)
+  (*         {| RealWorld.key_heap := A__keys; *)
+  (*            RealWorld.protocol := *)
+  (*              (m' <- @RealWorld.Recv (RealWorld.Pair RealWorld.Nat RealWorld.CipherId) (RealWorld.Signed KID2 RealWorld.Accept); *)
+  (*               RealWorld.Return *)
+  (*                 match RealWorld.unPair m' with *)
+  (*                 | Some (RealWorld.Plaintext n', _) => if n ==n n' then true else false *)
+  (*                 | _ => false *)
+  (*                 end)%realworld |}) $+ (B, *)
+  (*         {| RealWorld.key_heap := B__keys; *)
+  (*            RealWorld.protocol := *)
+  (*              (m <- RealWorld.Recv (RealWorld.Signed KID1 RealWorld.Accept); *)
+  (*               v <- RealWorld.Verify (RealWorld.AsymKey KEY1 false) m; *)
+  (*               m' <- match RealWorld.unPair m with *)
+  (*                    | Some (p, _) => RealWorld.Sign KEY__B p *)
+  (*                    | None => RealWorld.Sign KEY__B (RealWorld.Plaintext 1) *)
+  (*                    end; _ <- RealWorld.Send A m'; RealWorld.Return v)%realworld |}) $+ (B, *)
+  (*         {| RealWorld.key_heap := B__keys $++ $0; *)
+  (*            RealWorld.protocol := *)
+  (*              (m <- RealWorld.Return (RealWorld.Signature (RealWorld.Plaintext n) cid1); *)
+  (*               v <- RealWorld.Verify (RealWorld.AsymKey KEY1 false) m; *)
+  (*               m' <- match RealWorld.unPair m with *)
+  (*                    | Some (p, _) => RealWorld.Sign KEY__B p *)
+  (*                    | None => RealWorld.Sign KEY__B (RealWorld.Plaintext 1) *)
+  (*                    end; _ <- RealWorld.Send A m'; RealWorld.Return v)%realworld |}); *)
+  (*         RealWorld.adversary := $0; *)
+  (*         RealWorld.univ_data := *)
+  (*           {| RealWorld.users_msg_buffer := *)
+  (*                $0 $+ (B, [Exm (RealWorld.Signature (RealWorld.Plaintext n) cid1)]) $- B; *)
+  (*              RealWorld.all_keys := KEYS; *)
+  (*              RealWorld.all_ciphers := cs $+ (cid1, RealWorld.Cipher cid1 KID1 (RealWorld.Plaintext n)) |} *)
+  (*      |} *)
+  (* . *)
+  (* Proof. *)
+  (*   intros; do 3 eexists. smash_universe. *)
+  (* Qed. *)
 
 End ExamplarProofs.
